New version of united mergesort-quicksort. Revived SplaySort and SelectionSort. Refactored list lemmas a bit.

MsQsUnited.v
@@ -4,6 +4,10 @@ Import ListNotations.
 Class MsArgs : Type :=
 {
     A : Type;
+
+    small : list A -> option (A * list A);
+    adhoc : list A -> list A;
+
     split : A -> list A -> list (list A);
     join : list (list A) -> list A;
 }.
@@ -11,25 +15,43 @@ Class MsArgs : Type :=
 Coercion A : MsArgs >-> Sortclass.
 
 Unset Guard Checking.
-Fixpoint ms (A : MsArgs) (l : list A) {struct l} : list A :=
+Fixpoint qms (A : MsArgs) (l : list A) {struct l} : list A :=
 match l with
     | [] => []
     | [x] => [x]
     | h :: t =>
         let ls := split h t in
-        let ls' := map (ms A) ls in
+        let ls' := map (qms A) ls in
           join ls'
+end.
+
+Fixpoint qms' (A : MsArgs) (l : list A) {struct l} : list A :=
+match small l with
+    | None        => adhoc l
+    | Some (h, t) => join (map (qms' A) (split h t))
 end.
 Set Guard Checking.
 
 Instance MsArgs_nat : MsArgs :=
 {
     A := nat;
+
+    small l :=
+      match l with
+          | [] => None
+          | h :: t => Some (h, t)
+      end;
+
+    adhoc := id;
+
     split h t :=
        [ filter (fun x => leb x h) t
        ; [h]
        ; filter (fun x => negb (leb x h)) t
        ];
+
     join := @concat nat
 }.
+
+Compute qms MsArgs_nat [3; 2; 1; 0].
 
